Phi_OO.thy
@@ -1,0 +1,343 @@
+theory Phi_OO
+  imports NuInstructions
+begin
+
+chapter \<open>Object Oriented Programming Model\<close>
+
+section \<open>Semantics & Fictions\<close>
+
+subsection \<open>Models\<close>
+
+subsubsection \<open>Type\<close>
+
+paragraph \<open>Algebra of Class Dependency\<close>
+
+datatype 'TY class_id = Class (name: string) (parents: \<open>'TY class_id list\<close>) (fields: \<open>'TY list\<close>)
+hide_const (open) name parents fields
+
+text \<open>Name of a class is not its identity but the name plus parents.
+  It simplifies the model by ensuring two identical classes have identical parents.\<close>
+
+fun parents_of_with_self
+  where \<open>parents_of_with_self (Class name parents fields) =
+            insert (Class name parents fields) (\<Union> (parents_of_with_self ` set parents))\<close>
+
+
+instantiation class_id :: (type) order begin
+
+definition \<open>less_eq_class_id C1 C2 \<longleftrightarrow> C2 \<in> parents_of_with_self C1\<close>
+definition \<open>less_class_id (C1::'a class_id) C2 \<longleftrightarrow> C1 \<le> C2 \<and> C1 \<noteq> C2\<close>
+
+instance proof
+  fix x y z :: \<open>'a class_id\<close>
+
+  have \<open>\<And>x y S. x \<in> parents_of_with_self y \<Longrightarrow> x \<noteq> y \<Longrightarrow> size_class_id S x < size_class_id S y\<close>
+  subgoal for x y S
+  apply (induct y arbitrary: x)
+  subgoal for name parents fields x
+    apply clarsimp
+    subgoal for z
+      apply (cases \<open>x = z\<close>)
+      apply (metis not_add_less1 not_less_eq size_list_estimation)
+      by (metis Suc_lessD Suc_mono size_list_estimation trans_less_add1) . . .
+  then have t1: \<open>\<And>x y. y \<in> parents_of_with_self x \<and> x \<in> parents_of_with_self y \<Longrightarrow> x = y\<close>
+    by (metis order_less_asym)
+  then  show \<open>(x < y) = (x \<le> y \<and> \<not> y \<le> x)\<close>
+    apply (simp_all add: less_eq_class_id_def less_class_id_def)
+    by blast
+
+  show \<open> x \<le> y \<Longrightarrow> y \<le> x \<Longrightarrow> x = y\<close>
+    by (simp add: less_eq_class_id_def less_class_id_def t1)
+
+  show \<open>x \<le> x\<close>
+    by (cases x; simp add: less_eq_class_id_def less_class_id_def)
+
+  show \<open>x \<le> y \<Longrightarrow> y \<le> z \<Longrightarrow> x \<le> z\<close>
+    unfolding less_eq_class_id_def less_class_id_def
+    by (induct x, auto)
+qed
+end
+
+lemma [simp]: \<open>x \<in> parents_of_with_self x\<close>
+  by (cases x, simp)
+
+lemma [simp]: \<open>Class name (x # L) fields \<noteq> x\<close>
+proof
+  assume \<open>Class name (x # L) fields = x\<close>
+  then have \<open>\<And>S. size_class_id S (Class name (x # L) fields) = size_class_id S x\<close> by simp
+  then show False by simp
+qed
+
+lemma prop_subclass_1[intro]: \<open>Class name (x#L) fields < x\<close>
+  unfolding less_class_id_def less_eq_class_id_def by simp
+
+lemma subclass_1[intro]: \<open>Class name (x#L) fields \<le> x\<close>
+  unfolding less_class_id_def less_eq_class_id_def by simp
+
+lemma subclass_0[intro]: \<open>x \<le> x\<close> for x :: \<open>'a class_id\<close> by simp
+
+(* TODO!
+ lemma [intro]: \<open>Class name L \<le> x \<Longrightarrow> Class name (y#L) \<le> x\<close>
+  unfolding less_class_id_def less_eq_class_id_def apply simp*)
+
+
+paragraph \<open>Main Stuff\<close>
+
+virtual_datatype \<phi>OO_ty = \<phi>min_ty +
+  T_ref :: unit
+
+context \<phi>OO_ty begin
+abbreviation \<open>\<tau>Ref \<equiv> T_ref.mk ()\<close>
+end
+
+
+subsubsection \<open>Value\<close>
+
+datatype 'TY object_ref = object_ref ("class": \<open>'TY class_id\<close>) ("nonce": nat) | Nil
+hide_const (open) "class" nonce
+
+primrec of_class
+  where \<open>of_class cls (object_ref cls' _) \<longleftrightarrow> cls = cls'\<close>
+     | \<open>of_class _ Nil \<longleftrightarrow> True\<close>
+
+virtual_datatype 'TY \<phi>OO_val :: "nonsepable_semigroup" = 'TY \<phi>min_val +
+  V_ref :: \<open>'TY object_ref\<close>
+
+
+subsubsection \<open>Resource\<close>
+
+type_synonym field_name = string
+type_synonym ('TY,'VAL) object_heap = \<open>('TY object_ref \<times> field_name \<Rightarrow> 'VAL option)\<close>
+
+resource_space ('VAL::"nonsepable_semigroup",'TY) \<phi>OO_res = ('VAL,'TY) \<phi>min_res +
+  R_objs :: \<open>('TY,'VAL) object_heap ?\<close>
+
+
+subsection \<open>Main Stuff of Semantics\<close>
+
+locale \<phi>OO_sem_pre =
+  \<phi>min_sem where TYPES = \<open>TYPE(('TY_N \<Rightarrow> 'TY)
+                  \<times> ('VAL_N \<Rightarrow> 'VAL::nonsepable_semigroup)
+                  \<times> ('RES_N \<Rightarrow> 'RES::comm_monoid_mult))\<close>
++ \<phi>OO_ty where CONS_OF   = TY_CONS_OF
+            and TYPE'NAME = \<open>TYPE('TY_N)\<close>
+            and TYPE'REP  = \<open>TYPE('TY)\<close>
++ \<phi>OO_val where CONS_OF   = VAL_CONS_OF
+            and TYPE'TY   = \<open>TYPE('TY)\<close>
+            and TYPE'NAME = \<open>TYPE('VAL_N)\<close>
+            and TYPE'REP  = \<open>TYPE('VAL::nonsepable_semigroup)\<close>
++ \<phi>OO_res where TYPE'VAL  = \<open>TYPE('VAL)\<close>
+            and TYPE'TY   = \<open>TYPE('TY)\<close>
+            and TYPE'NAME = \<open>TYPE('RES_N)\<close>
+            and TYPE'REP  = \<open>TYPE('RES::comm_monoid_mult)\<close>
++ fixes TYPES :: \<open>(('TY_N \<Rightarrow> 'TY)
+                \<times> ('VAL_N \<Rightarrow> 'VAL::nonsepable_semigroup)
+                \<times> ('RES_N \<Rightarrow> 'RES::comm_monoid_mult)
+            ) itself\<close>
+assumes WT_ref[simp]: \<open>Well_Type \<tau>Ref = UNIV\<close>
+  and   zero_ref[simp]: \<open>Zero \<tau>Ref = V_ref.mk Nil\<close>
+  and   type_measure_ref[simp]:  \<open>type_measure \<tau>Ref = 1\<close>
+  and   Can_EqCompare_ref[simp]: \<open>Can_EqCompare res (V_ref.mk ref1) (V_ref.mk ref2)\<close>
+  and   EqCompare_ref[simp]:     \<open>EqCompare (V_ref.mk ref1) (V_ref.mk ref2) \<longleftrightarrow> ref1 = ref2\<close>
+begin
+
+lemma Valid_Type_Ref[simp]:
+  \<open>Valid_Type \<tau>Ref\<close>
+  unfolding Inhabited_def by simp
+
+lemma objref_infinite_cls:
+  \<open>infinite {a. object_ref.class a = cls}\<close>
+  using inj_on_finite[where A = \<open>UNIV::nat set\<close> and B = \<open>{a. object_ref.class a = cls}\<close>
+        and f = \<open>\<lambda>n. object_ref cls n\<close>]
+  using inj_def by fastforce
+
+
+definition Valid_Objs :: "('TY,'VAL) object_heap set"
+  where "Valid_Objs = {h. \<forall>k. h (Nil,k) = None}"
+
+lemma Valid_Objs_1[simp]: \<open>1 \<in> Valid_Objs\<close>
+  unfolding Valid_Objs_def one_fun_def one_fine_def by simp
+
+lemma ObjHeap_freshness:
+  \<open>finite (dom f) \<Longrightarrow> \<exists>k. f k = 1 \<and> object_ref.class k = cls\<close>
+  unfolding dom_def
+  by (metis (mono_tags, lifting) finite_subset mem_Collect_eq objref_infinite_cls one_option_def subsetI)
+
+subsection \<open>Fictions\<close>
+
+definition \<open>fiction_objs I = Fiction (\<lambda>x. { 1(R_objs #= Fine y) |y. y \<in> \<I> I x })\<close>
+lemma fiction_objs_\<I>:
+  "\<I> (fiction_objs I) = (\<lambda>x. { 1(R_objs #= Fine y) |y. y \<in> \<I> I x})"
+  unfolding fiction_objs_def
+  by (rule Fiction_inverse) (auto simp add: Fictional_def one_set_def one_fine_def)
+
+definition \<open>share_val_fiction =
+      Fiction (\<lambda>m. {f. to_share o f = m})\<close>
+lemma share_val_fiction_\<I>:
+  \<open>\<I> share_val_fiction = (\<lambda>m. {f. to_share o f = m})\<close>
+  unfolding share_val_fiction_def
+  by (rule Fiction_inverse, simp add: Fictional_def one_set_def)
+
+definition "share_objs = fiction_objs (fiction.fine share_val_fiction)"
+
+end
+
+
+locale \<phi>OO_sem =
+  \<phi>OO_sem_pre where TYPES = \<open>TYPE(('TY_N \<Rightarrow> 'TY)
+                  \<times> ('VAL_N \<Rightarrow> 'VAL::nonsepable_semigroup)
+                  \<times> ('RES_N \<Rightarrow> 'RES::comm_monoid_mult))\<close>
++ fixes TYPES :: \<open>(('TY_N \<Rightarrow> 'TY) \<times> ('VAL_N \<Rightarrow> 'VAL) \<times> ('RES_N \<Rightarrow> 'RES)) itself\<close>
+assumes res_valid_objects[simp]: \<open>Resource_Validator R_objs.name = R_objs.inject ` Fine ` Valid_Objs\<close>
+begin
+end
+
+
+
+fiction_space (in \<phi>OO_sem) \<phi>OO_fic :: \<open>'RES_N \<Rightarrow> 'RES\<close> = \<phi>min_fic +
+  FIC_OO_share :: share_objs
+
+locale \<phi>OO =
+  \<phi>OO_fic where TYPES = \<open>TYPE(('TY_N \<Rightarrow> 'TY)
+                  \<times> ('VAL_N \<Rightarrow> 'VAL::nonsepable_semigroup)
+                  \<times> ('RES_N \<Rightarrow> 'RES::comm_monoid_mult))\<close>
+      and TYPE'NAME = \<open>TYPE('FIC_N)\<close>
+      and TYPE'REP = \<open>TYPE('FIC::{no_inverse,comm_monoid_mult})\<close>
++ \<phi>min where TYPES = \<open>TYPE(('TY_N \<Rightarrow> 'TY)
+                  \<times> ('VAL_N \<Rightarrow> 'VAL::nonsepable_semigroup)
+                  \<times> ('RES_N \<Rightarrow> 'RES::comm_monoid_mult)
+                  \<times> ('FIC_N \<Rightarrow> 'FIC))\<close>
++ fixes TYPES :: \<open>(('TY_N \<Rightarrow> 'TY) \<times> ('VAL_N \<Rightarrow> 'VAL) \<times> ('RES_N \<Rightarrow> 'RES) \<times> ('FIC_N \<Rightarrow> 'FIC)) itself\<close>
+begin
+
+lemma R_objs_valid_split: \<open>res \<in> Valid_Resource \<longleftrightarrow>
+    R_objs.clean res \<in> Valid_Resource \<and> (\<exists>m. res R_objs.name = R_objs.inject (Fine m) \<and> m \<in> Valid_Objs)\<close>
+  by (subst R_objs.split, simp add: Valid_Resource_def times_fun_def image_iff one_fine_def, blast)
+
+lemma R_objs_valid_split': \<open>NO_MATCH (R_objs.clean res') res \<Longrightarrow> res \<in> Valid_Resource \<longleftrightarrow>
+    R_objs.clean res \<in> Valid_Resource \<and> (\<exists>m. res R_objs.name = R_objs.inject (Fine m) \<and> m \<in> Valid_Objs)\<close>
+  using R_objs_valid_split .
+
+end
+
+
+section \<open>\<phi>Types\<close>
+
+subsection \<open>Reference\<close>
+
+context \<phi>OO_sem begin
+
+definition Ref :: \<open>'TY class_id \<Rightarrow> ('VAL, 'TY object_ref) \<phi>\<close>
+  where \<open>Ref cls ref = ({ V_ref.mk ref } \<^bold>s\<^bold>u\<^bold>b\<^bold>j of_class cls ref)\<close>
+
+lemma \<phi>Ref_expns[\<phi>expns]:
+  \<open>v \<in> (ref \<Ztypecolon> Ref cls) \<longleftrightarrow> v = V_ref.mk ref \<and> of_class cls ref\<close>
+  unfolding Ref_def \<phi>Type_def by (simp add: \<phi>expns)
+
+lemma \<phi>Ref_inhabited[\<phi>reason_elim!, elim!]:
+  \<open>Inhabited (ref \<Ztypecolon> Ref cls) \<Longrightarrow> (of_class cls ref \<Longrightarrow> C) \<Longrightarrow> C\<close>
+  unfolding Inhabited_def by (simp add: \<phi>expns)
+
+lemma \<phi>Ref_zero[\<phi>reason 1000]:
+  \<open>\<phi>Zero \<tau>Ref (Ref cls) Nil\<close>
+  unfolding \<phi>Zero_def by (simp add: \<phi>expns)
+
+lemma \<phi>Ref_eq[\<phi>reason 1000]:
+  \<open>\<phi>Equal (Ref cls) (\<lambda>_ _. True) (=)\<close>
+  unfolding \<phi>Equal_def by (simp add: \<phi>expns)
+
+lemma \<phi>Ref_semty[\<phi>reason 1000]:
+  \<open>\<phi>SemType (ref \<Ztypecolon> Ref cls) \<tau>Ref\<close>
+  unfolding \<phi>SemType_def by (simp add: \<phi>expns)
+
+end
+
+subsection \<open>Field\<close>
+
+definition \<phi>Field :: \<open>field_name \<Rightarrow> ('v, 'x) \<phi> \<Rightarrow> (field_name \<Rightarrow> 'v option, 'x) \<phi>\<close>
+  where \<open>\<phi>Field field T x = { 1(field \<mapsto> v) |v. v \<in> (x \<Ztypecolon> T) }\<close>
+
+lemma \<phi>Field_expns[\<phi>expns]:
+  \<open>p \<in> (x \<Ztypecolon> \<phi>Field field T) \<longleftrightarrow> (\<exists>v. p = 1(field \<mapsto> v) \<and> v \<in> (x \<Ztypecolon> T))\<close>
+  unfolding \<phi>Field_def \<phi>Type_def by simp
+
+lemma [\<phi>reason_elim!, elim!]:
+  \<open>Inhabited (x \<Ztypecolon> \<phi>Field field T) \<Longrightarrow> (Inhabited (x \<Ztypecolon> T) \<Longrightarrow> C) \<Longrightarrow> C\<close>
+  unfolding Inhabited_def by (simp add: \<phi>expns)
+
+subsection \<open>Object\<close>
+
+context \<phi>OO begin
+
+definition \<phi>Object :: \<open>'TY object_ref \<Rightarrow> (field_name \<Rightarrow> 'VAL share option, 'x) \<phi> \<Rightarrow> ('FIC_N \<Rightarrow> 'FIC, 'x) \<phi>\<close>
+  where \<open>\<phi>Object obj T x = { FIC_OO_share.mk (Fine (case_prod (1(obj := v)))) |v. v \<in> (x \<Ztypecolon> T) }\<close>
+
+lemma \<phi>Object_expn[\<phi>expns]:
+  \<open>p \<in> (x \<Ztypecolon> \<phi>Object obj T) \<longleftrightarrow> (\<exists>v. p = FIC_OO_share.mk (Fine (case_prod (1(obj := v)))) \<and> v \<in> (x \<Ztypecolon> T))\<close>
+  unfolding \<phi>Object_def \<phi>Type_def by simp
+
+lemma [\<phi>reason_elim!, elim!]:
+  \<open>Inhabited (x \<Ztypecolon> \<phi>Object obj T) \<Longrightarrow> (Inhabited (x \<Ztypecolon> T) \<Longrightarrow> C) \<Longrightarrow> C\<close>
+  unfolding Inhabited_def by (simp add: \<phi>expns)
+
+
+
+
+
+
+section \<open>Instructions\<close>
+
+definition \<phi>M_getV_ref :: \<open>'VAL sem_value \<Rightarrow> ('TY object_ref \<Rightarrow> ('ret,'RES_N,'RES) proc) \<Rightarrow> ('ret,'RES_N,'RES) proc\<close>
+  where \<open>\<phi>M_getV_ref v F = \<phi>M_getV \<tau>Ref V_ref.dest v F\<close>
+
+(*
+definition \<phi>M_obj_allocate :: \<open>'TY class_id \<Rightarrow> ('TY object_ref \<Rightarrow> ('ret,'RES_N,'RES) proc) \<Rightarrow> ('ret,'RES_N,'RES) proc\<close>
+  where \<open>\<phi>M_obj_allocate cls F = \<close>
+
+definition op_obj_new :: \<open>'TY class_id \<Rightarrow> ('VAL,'RES_N,'RES) proc\<close>
+  where \<open>op_obj_new cls = \<close> *)
+
+definition op_obj_load_field :: \<open>field_name \<Rightarrow> 'TY \<Rightarrow> ('VAL,'VAL,'RES_N,'RES) proc'\<close>
+  where \<open>op_obj_load_field field TY v =
+    \<phi>M_getV_ref v (\<lambda>ref.
+    \<phi>M_get_res_entry R_objs.get (ref,field) (\<lambda>v.
+    \<phi>M_assert (v \<in> Well_Type TY) \<ggreater> Success (sem_value v)))\<close>
+
+definition op_obj_store_field :: \<open>field_name \<Rightarrow> 'TY \<Rightarrow> ('VAL \<times> 'VAL, unit,'RES_N,'RES) proc'\<close>
+  where \<open>op_obj_store_field field TY =
+    \<phi>M_caseV (\<lambda>vstore vref.
+    \<phi>M_getV TY id vstore (\<lambda>store.
+    \<phi>M_getV_ref vref (\<lambda>ref.
+    \<phi>M_get_res_entry R_objs.get (ref,field) (\<lambda>v. \<phi>M_assert (v \<in> Well_Type TY))
+ \<ggreater> \<phi>M_set_res R_objs.updt (\<lambda>f. f((ref,field) \<mapsto> store))
+)))\<close>
+
+
+
+
+lemma (in \<phi>OO) \<phi>M_getV_ref[\<phi>reason!]:
+  \<open> \<^bold>p\<^bold>r\<^bold>o\<^bold>c F ref \<lbrace> X \<longmapsto> Y \<^bold>t\<^bold>h\<^bold>r\<^bold>o\<^bold>w\<^bold>s E \<rbrace>
+\<Longrightarrow> \<^bold>p\<^bold>r\<^bold>o\<^bold>c \<phi>M_getV_ref raw F \<lbrace> X\<heavy_comma> ref \<Ztypecolon> Val raw (Ref cls) \<longmapsto> Y \<^bold>t\<^bold>h\<^bold>r\<^bold>o\<^bold>w\<^bold>s E \<rbrace>\<close>
+  unfolding \<phi>M_getV_ref_def by (cases raw, simp, \<phi>reason, simp add: \<phi>expns)
+
+lemma (in \<phi>OO) op_obj_load_field:
+  \<open>\<^bold>p\<^bold>r\<^bold>o\<^bold>c op_obj_load_field field TY raw \<lbrace>
+      v \<Ztypecolon> \<phi>Object ref (\<phi>Field field (\<phi>Share n Identity)) \<heavy_comma> ref \<Ztypecolon> Val raw (Ref cls)
+  \<longmapsto> v \<Ztypecolon> \<phi>Object ref (\<phi>Field field (\<phi>Share n Identity)) \<heavy_comma> \<^bold>v\<^bold>a\<^bold>l v \<Ztypecolon> Identity
+\<rbrace>\<close>
+  unfolding op_obj_load_field_def
+  apply \<phi>reason
+  unfolding \<phi>M_get_res_entry_def \<phi>M_get_res_def \<phi>Procedure_def
+  apply (clarsimp simp add: \<phi>expns FIC_OO_share.interp_split' R_objs_valid_split' share_objs_def
+            fiction_objs_\<I> mult_strip_fine_011 R_objs.mult_strip_inject_011 share_val_fiction_\<I>
+            Valid_Objs_def times_fun)
+  
+
+apply (auto simp add: \<phi>expns FIC_mem.interp_split' R_mem_valid_split' times_fun dom_mult
+                        R_mem.mult_in_dom Valid_Mem_def mult_strip_fine_011 mult_strip_fine_001
+                        fiction_mem_\<I>'' share_mem_def' times_list_def)
+end
+
+
+
+end
